ProtoSynthDataTypeEqualities.v
@@ -1,0 +1,85 @@
+Add LoadPath "/users/paulkline/Documents/coqs/protosynth". 
+Require Import MyShortHand. 
+Require Export ProtoSynthDataTypes.
+Require Import ProtoSynthProtocolDataTypes.
+Require Import Coq.Program.Equality.
+Create HintDb eq_dec_db.
+
+(*Nouns *)
+Theorem eq_dec_noun : forall n1 n2 : Noun, {n1 = n2} + {n1 <> n2}.
+Proof. intros;  destruct n1, n2; 
+  try (left;reflexivity); right; unfold not; intros H; inversion H.
+Defined.
+Hint Resolve eq_dec_noun : eq_dec_db.
+
+(*Attributes *)
+Theorem eq_dec_attribute : forall a1 a2 : Attribute,
+                    {a1 = a2} + {a1 <> a2}.
+Proof. decide equality; rec_eq.
+Defined. 
+Hint Resolve eq_dec_attribute : eq_dec_db. 
+
+(*DescriptionR *)
+Theorem eq_dec_DescriptionR1 : 
+forall n : Noun,
+forall a : Attribute,
+forall x y : DescriptionR n a,
+x = y.
+Proof. intros;
+induction x; dependent induction y;
+( reflexivity).
+Defined.
+Hint Resolve eq_dec_DescriptionR1 : eq_dec_db.
+
+Theorem eq_dec_Description : 
+forall d1 d2 : Description,
+{d1 = d2} + {d1 <> d2}. 
+Proof. intros. destruct d1, d2.   
+specialize eq_dec_attribute with a a0. intros. destruct H.
+ specialize eq_dec_noun with n n0. intros.
+destruct H. left. subst. specialize eq_dec_DescriptionR1 with n0 a0 d0 d.
+intros. subst. reflexivity.
+right. unfold not. intros. inversion H. contradiction.
+right. unfold not. intros. inversion H. contradiction.
+Defined. 
+Hint Resolve eq_dec_Description : eq_dec_db.
+
+Theorem eq_dec_bool : forall b c : bool, 
+{b = c} + {b <> c}.
+decide equality.
+Defined.
+Hint Resolve  eq_dec_bool : eq_dec_db.
+
+Require Import FunctionalExtensionality. 
+Theorem eq_dec_f {A} {B} : forall (a b : (A -> B)), a =<> b.
+Proof. intros. Admitted.
+
+Theorem eq_dec_Requirement : forall d (x y : Requirement d), x =<> y.
+Proof. intros. destruct d, x, y,d; simpl in b, b0; destruct (eq_dec_f b b0); eqdecHelper.  
+Qed.
+Hint Resolve eq_dec_Requirement : eq_dec_db.
+
+Theorem eq_dec_Action : forall x y : Action,
+{x = y} + {x <>y }.
+Proof. decide equality. Defined.
+Hint Resolve  eq_dec_Action : eq_dec_db.
+
+
+
+Theorem eq_dec_RequestItem : forall x y : RequestItem,
+ {x = y} + {x <> y}. Proof. intros. destruct x,y. destruct (eq_dec_Description d d0); subst. (destruct r, r0).  eauto. destruct (eq_dec_f b b0);subst. eqdecHelper. destruct d0. simpl in b0,b. destruct d. simpl.
+Admitted.
+
+Theorem eq_dec_Role: forall x y : Role, {x = y} + {x <> y}. 
+Proof. decide equality. Defined.
+Hint Resolve eq_dec_Role. 
+
+Theorem eq_dec_VarID : forall x y : VarID, {x = y} + {x <> y}.
+Proof. intros. destruct x,y; 
+  (left; reflexivity) || 
+  (decide equality; rec_eq) ||
+  (right; unfold not;intros;inversion H).
+Defined.
+
+Theorem eq_dec_Participant : forall x y : Participant, {x = y} + {x <> y}.
+ Proof. decide equality. Defined.
