ProtoSynthDataTypes.v
@@ -1,0 +1,81 @@
+Add LoadPath "/users/paulkline/Documents/coqs/protosynth". 
+Require Import MyShortHand.
+
+Inductive Noun : Set:=
+  | VirusChecker
+  | PCR.
+
+(* Now we define what it is we would like to know about these nouns. *)
+Inductive Attribute : Set :=
+  | Name : Attribute
+  | Hash : Attribute
+  | Index : nat -> Attribute
+  | Version : Attribute.
+
+(*We only want to disallow nonsensical combinations, like a (PCR, version),
+ hence this relation. *)
+Inductive DescriptionR : Noun -> Attribute -> Set :=
+  | pcrMR : forall n, DescriptionR PCR (Index n)
+  | virusCheckerNameR : DescriptionR VirusChecker Name
+  | virusCheckerVersionR : DescriptionR VirusChecker Version.
+
+(* This 'extra step' is done simply so that comparison between descriptors
+is 'easy.'It is much more involved to be able to compare indexed types. *)
+Inductive Description : Set :=
+  | descriptor {n : Noun} {a : Attribute} : DescriptionR n a -> Description.
+
+
+(*This defines what the type of measuring these things should be. *)
+Definition measurementDenote (d: Description) :=
+match d with
+ | descriptor r => (match r with
+    | pcrMR n => nat
+    | virusCheckerNameR => nat
+    | virusCheckerVersionR => bool
+    end)
+end.
+
+(* Here we begin specificiation of requirements. So not only do I want a particular measurment,
+   but I want it to be certain values. *) 
+Inductive Requirement (d : Description) :=
+| requirement : ( (measurementDenote d) -> bool) -> Requirement d.
+
+
+(* This begins the defining of what a privacy policy is. First we define a rule.
+    A rule regulates the release of a measurement. We could decide to release information if
+    some counter condition holds; we could release it for free; we could explicitly never release it; 
+    or some combination of and-ing and or-ing rules.
+    Note that at this point we've allowed for nonsensical release rules like, "never release or release for free",
+     "release for free and never release".
+    NOTE: If we can't request something twice, what if duplicate occurs in rule req?
+          todo: keep all received measurements and check those first for the value *) 
+Inductive Rule (mything : Description) :=  
+| rule  {your : Description} : (Requirement your) -> Rule mything
+| free : Rule mything
+| never : Rule mything
+| multiReqAnd : Rule mything ->Rule mything -> Rule mything
+| multiReqOr : Rule mything -> Rule mything -> Rule mything.
+
+(* simply a list of rules. *)
+Inductive PrivacyPolicy :=
+| EmptyPolicy : PrivacyPolicy
+| ConsPolicy {d :Description}: 
+    Rule d -> 
+    PrivacyPolicy -> PrivacyPolicy.
+
+Inductive Action : Set :=
+ | ASend : Action
+ | AReceive : Action.
+
+(*A RequestItem is used to compose a list of the items and requirements upon 
+those items in an attestation *)
+Inductive RequestItem : Set :=
+ | requestItem (d : Description) : (Requirement d) -> RequestItem.
+
+Inductive RequestLS : Set :=
+ | emptyRequestLS : RequestLS
+ | ConsRequestLS : RequestItem -> RequestLS -> RequestLS.
+
+Inductive Role : Set :=
+ | Appraiser
+ | Attester.
