ProtoSynthProtocolDataTypes.v
@@ -1,0 +1,83 @@
+Add LoadPath "/users/paulkline/Documents/coqs/protosynth". 
+Require Import MyShortHand.
+Require Import ProtoSynthDataTypes.
+
+Inductive VarID :=
+ | receivedMESSAGE : VarID
+ | toSendMESSAGE : VarID
+ | variden : nat -> VarID.
+
+Inductive Const :=
+ | constValue (d: Description) : (measurementDenote d) -> Const 
+ | constRequest : Description -> Const
+ | constStop : Const
+ | constNULL : Const
+ | constMeasurementPlaceHolder : Const.
+
+Inductive Term :=
+ | variable : VarID -> Term
+ | const : Const -> Term.
+
+Inductive Condition :=
+ | IsMyTurntoSend : Condition
+ | QueuedRequestsExist : Condition
+ | ExistsNextDesire : Condition
+ | CanSend :  Condition
+ | IsSend :  Condition
+ | IsMeasurement : Term -> Condition
+ | IsRequest : Term -> Condition
+ | IsStop : Term -> Condition
+ | IsAllGood : Condition.
+
+Inductive AllGood :=
+ | Yes
+ | No
+ | Unset.
+
+Inductive Computation := 
+ | compGetMessageToSend
+ | compGetNextRequest
+ | compGetfstQueue.
+
+Inductive Effect :=
+ | effect_StoreRequest : Term -> Effect
+ | effect_ReduceStatewithMeasurement : Term -> Effect
+ | effect_ReducePrivacyWithRequest : Term -> Effect
+ | effect_MvFirstDesire :  Effect
+ | effect_rmFstQueued : Effect
+ | effect_cp_ppUnresolved : Term -> Effect
+ | effect_setAllGood : AllGood -> Effect.
+
+Inductive Participant :=
+ | ATTESTER
+ | APPRAISER.
+
+Inductive Statement :=
+ | SendStatement : Term -> Participant -> Participant -> Statement
+ | ReceiveStatement : VarID -> Statement
+ | EffectStatement : Effect -> Statement
+ | Compute : VarID -> Computation -> Statement
+ | Assignment : VarID -> Term -> Statement
+ | Choose : Condition -> Statement -> Statement -> Statement
+ | Chain : Statement -> Statement -> Statement
+ | StopStatement : Statement
+ | EndStatement : Statement
+ | Skip : Statement
+ | Wait : Statement.
+
+Notation "'IFS' x 'THEN' y 'ELSE' z" := (Choose x y z)(at level 80, right associativity). 
+Notation "x '>>' y" := (Chain x y)  (at level 60, right associativity).
+
+Definition VarState := list (VarID*Const).
+ 
+Inductive ProState :=
+ (*  action <who am I?> privacyPol <things I want to ask for!> <Things I've asked for and am waiting for a response> tosend *)
+ | proState : Action -> AllGood -> Participant ->  PrivacyPolicy -> RequestLS -> RequestLS -> list Description
+      -> ProState.
+      
+Inductive State :=
+ state : VarState -> ProState -> State.
+
+Inductive NetworkMessage :=
+ networkMessage : Participant -> Participant -> Const -> NetworkMessage. 
+Definition Network := list NetworkMessage.
